io/case-study/WebServer.Compiled.fst
@@ -1,29 +1,66 @@
 module WebServer.Compiled
 
+open FStar.Ghost
 open FStar.Tactics
 open FStar.List.Tot
 
-open Common
-open Shared
+open Compiler.Model
 open WebServer
-open ILang.CompileTo.Tot
 
-(** TODO: can these two steps be combined? **)
-val compiled_webserver : plugin_type -> IIOwp (maybe unit) (trivial_hist ())
+let check_send_pre : tree pck_rc = 
+  Node 
+    (| Bytes.bytes, unit, (fun msg h _ _ -> (Bytes.length msg) < 500) |)
+    Leaf
+    Leaf
+
+let export_send (#fl:erased tflag) : exportable ((msg:Bytes.bytes -> IIO (resexn unit) fl (fun h -> Bytes.length msg < 500)
+                                            (fun _ _ lt -> exists fd r. lt == [EWrite true (fd,msg) r] ))) Utils.pi check_send_pre fl =
+  exportable_arrow_pre_post_args Bytes.bytes unit
+    (fun msg h ->  Bytes.length msg < 500)
+    (fun msg _ _ lt -> exists fd r. lt == [EWrite true (fd,msg) r])
+    #()
+    #()
+
+
+let check_handler_post : tree pck_rc =
+  Node (| file_descr, resexn unit, (fun client _ _ lt -> Utils.wrote_at_least_once_to client lt) |)
+    check_send_pre 
+    Leaf
+
+(* Breaks F* *)
+instance import_request_handler (fl:erased tflag) : safe_importable (req_handler fl) Utils.pi check_handler_post fl = admit ()
+(* {
+  swtyp = file_descr -> Bytes.bytes -> export_send.wtyp -> IIOpi (resexn unit) fl Utils.pi;
+  c_swtyp = weak_arrow3 fl Utils.pi file_descr Bytes.bytes export_send.wtyp #export_send.c_wtyp(resexn unit);
+  safe_import = (fun (f:file_descr -> Bytes.bytes -> export_send.wtyp -> IIOpi (resexn unit) fl Utils.pi) eff_rcs -> 
+    let f' : req_handler fl = (fun fd req -> 
+      let f'' = f fd req in
+      (safe_importable_arrow_pre_post_res 
+        #_ #_
+        #Utils.pi
+        #check_handler_post
+        #fl
+        (fun _ _ -> True)
+        (fun _ h r lt -> enforced_locally Utils.pi h lt /\ 
+          (Utils.wrote_at_least_once_to fd lt \/ Inr? r))
+        ((fun () -> admit ()) ())
+        ((fun () -> admit ()) ())
+        #export_send).safe_import f'' eff_rcs) in
+    f'
+  )
+}*)
+
+
+let interface : src_interface = {
+  pi = Utils.pi;
+  phi = Utils.phi;
+  ct = req_handler;
+  ct_rcs = check_handler_post;
+  ct_importable = (fun fl -> import_request_handler fl); 
+  psi = (fun _ _ lt -> Utils.every_request_gets_a_response lt);
+}
+
 let compiled_webserver = 
-  simpl_trivialize
-    (fun _ _ -> true)
-    (fun _ h r lt -> iio_post shr.pi h r lt)
-    webserver
+  comp.compile_pprog #interface webserver 
 
-let webserver_mlify = 
-  mlifyable_inst_iiowp
-    plugin_type 
-    (maybe unit)
-    #(instrumentable_IIO #shr.ctx_arg #shr.ctx_ret #ml_file_descr shr.pre shr.post shr.pi #shr.post_c) 
-    #(ml_maybe unit)
-
-let compiled_webserver'' : (Types.file_descr -> Tot (maybe unit)) -> ML (maybe unit) =
-  (mlify #_
-    #webserver_mlify
-    compiled_webserver)
+(** TODO: compile webserver to ML/Tot **)
